\documentclass[12pt,letterpaper]{article}

\usepackage{fancyhdr,fancybox}

\input{tskpreamble_nothms} %find me at /home/trevor/texmf/tex/latex/tskpreamble_nothms.tex
\input{tsktheoremstyles}

%%
%% Page set-up:
%%
\pagestyle{empty}
\lhead{\textsc{201 - Real Analysis \\}} 
\rhead{\textsc{Harutyunyan, Winter 2020} \\ Trevor Klar}
%\chead{\Large\textbf{A New Integration Technique \\ }}
\renewcommand{\headrulewidth}{0pt}
%
\renewcommand{\footrulewidth}{0pt}
%\lfoot{
%Office: \quad \quad \, M 2-3 \, \, SH 6431x \\
%Math Lab: \, W 12-2 \, SH 1607
%}
%\rfoot{trevorklar@math.ucsb.edu}

\setlength{\parindent}{0in}
\setlength{\textwidth}{7in}
\setlength{\evensidemargin}{-0.25in}
\setlength{\oddsidemargin}{-0.25in}
\setlength{\parskip}{.5\baselineskip}
\setlength{\topmargin}{-0.5in}
\setlength{\textheight}{9in}

\setlist[enumerate,1]{label=\textbf{\arabic*.}}

\renewcommand{\phi}{\varphi}
\renewcommand{\epsilon}{\varepsilon}

\begin{document}
\pagestyle{fancy}
\begin{center}
{\Large Homework 3}%=================UPDATE THIS=================%
\end{center}

\jpg{width=\linewidth}{hw3-p1-1}
\begin{proof}
Let $\mu$ denote the Lebesgue measure. %\WLOG{} suppose $f(x)\geq0$ for all $x\in [0,1]$. 
Since $f$ is a continuous function on a compact set, then it is uniformly continuous. Given $\epsilon>0$, choose $\delta$ according to the uniform continuity of $f$. Let 
$$g_\epsilon (x) := f(n\delta), \text{ where $n\in \N$ is such that } n\delta\leq x<(n+1)\delta.$$
This means that for any $x\in [0,1]$ we have $\abs{ x-n\delta}<\delta$, so $\abs{f(x)-g_\epsilon(x)}=\abs{f(x)-f(n\delta)}<\epsilon$. Furthermore, $g_\epsilon$ is a simple function, so $g'_\epsilon=0$ \muae{} and we are done. 
\end{proof}

\jpg{width=\linewidth}{hw3-p4-1}
\begin{lemma}
For $a,b\geq0$, $p\geq1$, 
$$(a+b)^p\leq a^p+(p)(2^{p-1})(a^{p-1}b+b^p).$$
\end{lemma}
\textsc{Proof of Lemma} Let $a\geq0$, $p\geq1$ and define 
$$\psi(t)=(a+t)^p- \big(a^p+(p)(2^{p-1})(a^{p-1}t+t^p)\big).$$
Observe that $\psi(0)=0$, and 
$$\psi'(t)=p\big((a+t)^{p-1}- (2^{p-1})(a^{p-1}+pt^{p-1})\big)$$
and clearly $(a+t)^{p-1} < (2^{p-1})(a^{p-1}+pt^{p-1})$, so $\psi(t)<0$ for all $t>1$ and the lemma is proved. \qedwhite
\begin{proof}To suppress notation, we write $\int f\dx$ to mean $\int_\R f(x)\dx$. 
We will show that $\phi$ is locally Lipschitz, and therefore differentiable. For all $t\in \R$ and $h\in(0,1)$, 
\begin{align*}
\frac{\abs{\phi(t)-\phi(t+h)}}{|h|}
&=\frac{1}{|h|}{\abs{\ds\int\abs{f+(t+h)g}^p\dx - \ds\int\abs{f+tg}^p\dx}} \\
&=\frac{1}{|h|}{\abs{\ds\int\abs{A+hg}^p\dx - \ds\int\abs{A}^p\dx}} &\text{where }A=f+tg\\
&\leq\frac{1}{|h|}{\abs{\ds\int\big|\abs{A}+\abs{hg}\big|^p\dx - \ds\int\abs{A}^p\dx}} \\
&\leq\frac{1}{|h|}{\abs{\ds\int|A|^p+(2^{p-1})(p)\left(|A|^{p-1}|hg|+|hg|^p\right)\dx - \ds\int\abs{A}^p\dx}} &\text{by the Lemma}\\
&=\frac{(2^{p-1})(p)}{|h|}{\abs{\ds\int|A|^{p-1}|hg|+|hg|^p\dx}} \\
&={(2^{p-1})(p)}{\abs{\ds\int|A|^{p-1}|g|+|h|^{p-1}|g|^p\dx}}. \\
\end{align*}
We know that $\int|h|^{p-1}|g|^p\dx\leq |g|^p\dx<\infty$ since $h\in(0,1)$ and $g\in L^p(\R)$, so we need to show that $\int|A|^{p-1}|g|\dx<\infty$. Now $p\geq 1$, so the conjugate exponent of $p$ is $q\frac{p}{p-1}$, so by Young's inequality we can write 
$$\int|A|^{p-1}|g|\dx=\int|g||A|^{p-1}\dx\leq \int\frac{|g|^p}{p}+\frac{|A|^{p}}{q}\dx.$$
We know that $\int\frac{|g|^p}{p}\dx<\infty$ since $g\in L^p(\R)$, so it still remains to show that $\int\frac{|A|^{p}}{q}\dx<\infty$. Note that the function $|\cdot|^p:\R\to\R$ is convex, so 
$$\int\frac{|A|^{p}}{q}\dx=\frac{1}{q}\int{|f+tg|^{p}}\dx\leq\frac{1}{q}\int{|f|^{p}+t|g|^{p}}\dx<\infty$$
since $f,g\in L^p(\R)$ and we're done. 
\end{proof}


\end{document}
