\documentclass[letterpaper]{article}
%\documentclass[a5paper]{article}

%% Language and font encodings
\usepackage[english]{babel}
\usepackage[utf8x]{inputenc}
\usepackage[T1]{fontenc}


%% Sets page size and margins
\usepackage[letterpaper,top=.75in,bottom=1in,left=1in,right=1in,marginparwidth=1.75cm]{geometry}
%\usepackage[a5paper,top=1cm,bottom=1cm,left=1cm,right=1.5cm,marginparwidth=1.75cm]{geometry}

\usepackage{graphicx}
%\graphicspath{../images}	  %%where to look for images

\input{../tskpreamble}

\pgfplotsset{compat=1.13}

%\newcommand{\T}{\mathcal{T}}
%\newcommand{\B}{\mathcal{B}}

%These commands are now in tskpreamble_nothms.tex, but are left as a comment here for reference. 
%\newcommand{\arbcup}[1]{\bigcup\limits_{\alpha\in\Gamma}#1_\alpha}
%\newcommand{\arbcap}[1]{\bigcap\limits_{\alpha\in\Gamma}#1_\alpha}
%\newcommand{\arbcoll}[1]{\{#1_\alpha\}_{\alpha\in\Gamma}}
%\newcommand{\arbprod}[1]{\prod\limits_{\alpha\in\Gamma}#1_\alpha}
%\newcommand{\finitecoll}[1]{#1_1, \ldots, #1_n}
%\newcommand{\finitefuncts}[2]{#1(#2_1), \ldots, #1(#2_n)}
%\newcommand{\abs}[1]{\left|#1\right|}
%\newcommand{\norm}[1]{\left|\left|#1\right|\right|}

\title{Math 450b \linebreak
Homework 8}
\author{Trevor Klar}

\begin{document}

\maketitle

\begin{enumerate}
\item Let $f:\R^n\to \R^n$ and suppose there is a constant $M$ such that $\norm{f(\vecb{x})}\leq M\norm{\vecb{x}}^2$ for all $\vecb{x}\in \R^n$. Let $g(\vecb{x})=T(\vecb{x})+f(\vecb{x})$, where $T:\R^n\to \R^n$ is an invertible linear transformation. Prove that $g$ is locally invertible near $\vecb{0} $. 
\begin{proof}
To prove that $g$ is locally invertible near $\vecb{0} $, we will show that $\det \left(Dg(\vecb{0})\right)\neq0$. Since
$$g(\vecb{x})=T(\vecb{x})+f(\vecb{x}),$$
Then by linearity of derivatives, 
\[\begin{array}{rcl}
Dg(\vecb{0})(\vecb{x})&=&DT(\vecb{0})(\vecb{x})+Df(\vecb{0})(\vecb{x})\\
&=&T(\vecb{x})+Df(\vecb{0})(\vecb{x})
\end{array}\]

By an earlier homework problem, since $\norm{f(\vecb{x})}\leq M\norm{\vecb{x}}^2$ for all $\vecb{x}\in \R^n$, then $Df(\vecb{0})\equiv\vecb{0}$. Thus, 
$$Dg(\vecb{0})(\vecb{x})=T(\vecb{x}),$$
ans since $T$ is invertible, $\det(Dg(\vecb{0}))=\det(T)\neq 0$. 
\end{proof}

\item Determine whether the system 
\[\begin{array}{rcl}
u &=& x+xyz\\
v &=& y+xy\\
w &=& z+2x+3z^2\\
\end{array}\]
can be solved for $x,y,z$ in terms of $u,v,w$ near $(0,0,0)$. 
\begin{proof}
Let $f:\R^3\to \R^3$ be defined as $f(x,y,z)=(u,v,w)$. Note that $f(\vecb{0})=\vecb{0}$. We seek some $\inv{f}(u,v,w)=(x,y,z)$ near $\vecb{0}$. If $\det(Df(\vecb{0}))\neq0$ (We can already can see that $f$ is continuous), then the Inverse Function Theorem guarantees the desired function. 
\[Df=\left[
\begin{array}{ccc}
1+yz & xz & xy\\
y & 1+x & 0\\
z & 0 & 1+6z\\
\end{array}\right]
\quad
Df(\vecb{0})=\left[
\begin{array}{ccc}
1&0&0\\
0&1&0\\
2&0&1\\
\end{array}\right]
\]
$Df(\vecb{0})$ is lower-triangular, so $\det Df(\vecb{0})=(1)(1)(1)\neq0$. Thus, $f$ is locally invertible near $\vecb{0}$ and we are done. 
\end{proof}

\item Suppose $f:U\subset \R^n\to \R^n$ is $C^1$ and one-to-one, with $Df(\vecb{a})\neq0$ for all $\vecb{a}\in U$. Prove that $f(U)$ is an open set. 
\begin{proof}
Let $\vecb{y}\in f(U)$ with $f(\vecb{x})=\vecb{y}$ for some $\vecb{x}\in U$. Since $\det(Df(\vecb{x}))\neq0$ by assumption, the Inverse Function Thm gives open sets $V, W$ such that 
$$\vecb{x}\in V \subset U, \quad \vecb{y}\in W \subset f(U),$$
thus $f(U)$ is open by the openness criterion. 
\end{proof}

\item Determine whether the system 
\[\begin{array}{rcl}
3x+2y+z^2+u+v^2 &=& 0\\
4x+3y+z+u^2+v+w+2 &=& 0\\
x+z+w+u^2+2 &=& 0\\
\end{array}\]
can be solved for $u,v,w$ in terms of $x,y,z$ near $x=y=z=u=v=0, w=-2$.
\begin{proof}
Denote the point $$x=y=z=u=v=0, w=-2$$ as $-2\vecb{e}_w$. Let $F:\R^6\to\R^3$ be defined as 
\[
F(x,y,z,u,v,w)=\left[
\begin{array}{c}
3x+2y+z^2+u+v^2\\
4x+3y+z+u^2+v+w+2\\
x+z+w+u^2+2\\
\end{array}\right]
\]
Observe that $F(-2\vecb{e}_w)=\vecb{0}$. If 
$$\det\left(\left[\frac{\del F_i}{\del j}(-2\vecb{e}_w)\right]_{\substack{i\in\{1,2,3\}\\j\in\{u,v,w\}}}\right)\neq0,$$
then the Implicit Function Theorem gives open sets $V_1\in \R^3, V_2\in \R^3$ with $\vecb{0}\in V_1$ and $(0,0,-2)\in V_2$, and some $f:V_1\to V_2$ such that $F(x,y,z,f(x,y,z))=\vecb{0}$ for all $(x,y)\in V_1$. Thus, we calculate the above determinant. 
\[
\det\left(\left[\frac{\del F_i}{\del j}(-2\vecb{e}_w)\right]_{\substack{i\in\{1,2,3\}\\j\in\{u,v,w\}}}\right)
=
\det\left(\left.\left[
\begin{array}{ccc}
1 & 2v & 0 \\
2u & 1 & 1 \\
2u & 0 & 1 \\
\end{array}
\right]\right|_{-2\vecb{e}_w}\right)
=
\left|\begin{array}{ccc}
1 & 0 & 0 \\
0 & 1 & 1 \\
0 & 0 & 1 \\
\end{array}\right|
=
1\neq0
\]
as desired, and we are done.
\end{proof}

\item Show that the equations 
\[\begin{array}{rcl}
x^2-y^2-u^3+v^2+4 &=& 0\\
2xy+y^2-2u^2+3v^4+8 &=& 0\\
\end{array}\]
determine functions $u(x,y), v(x,y)$ near $x=2, y=-1$ such that $u(2,-1)=2$, $v(2,-1)=1$. Compute $\frac{\del u}{\del x}$. 

\begin{proof}
Let $F:\R^4\to\R^2$ be defined as 
\[
F(x,y,u,v)=\left[
\begin{array}{c}
x^2-y^2-u^3+v^2+4\\
2xy+y^2-2u^2+3v^4+8\\
\end{array}\right]_.
\]
Observe that $F(2,-1,2,1)=\vecb{0}$. If 
$$\det\left(\left[\frac{\del F_i}{\del j}(2,-1,2,1)\right]_{\substack{i\in\{1,2\}\\j\in\{u,v\}}}\right)\neq0,$$
then the Implicit Function Theorem gives open sets $V_1\in \R^2, V_2\in \R^2$ with $(2,-1)\in V_1$ and $(2,1)\in V_2$, and some $f:V_1\to V_2$ such that $F(x,y,f(x,y))=F(x,y,u(x,y),v(x,y))=\vecb{0}$ for all $(x,y)\in V_1$. Thus, we calculate the above determinant. 
\[
\det\left(\left[\frac{\del F_i}{\del j}(2,-1,2,1)\right]_{\substack{i\in\{1,2\}\\j\in\{u,v\}}}\right)
=
\det\left(\left.\left[
\begin{array}{ccc}
-3u^2 & 2v \\
-4u & 12v^3 \\
\end{array}
\right]\right|_{(2,-1,2,1)}\right)
=
\left|\begin{array}{ccc}
-12 & 2 \\
-8 & 12 \\
\end{array}\right|
=
-144+16\neq0
\]
as desired, and we are done.
\end{proof}
\textbf{Solution} Now we calculate $\frac{\del u}{\del x}$ by differentiating $F(x,y,u,v)=\vecb{0}$ implicitly. 
\[
\frac{\del}{\del x}
\left[\begin{array}{c}
x^2-y^2-u^3+v^2+4\\
2xy+y^2-2u^2+3v^4+8\\
\end{array}\right]
=
\frac{\del}{\del x}
\left[\begin{array}{c}
0\\
0\\
\end{array}\right]
\]
This gives the following system of equations, if we consider $u$ and $v$ to be functions of $x$ but $y$ to be constant with respect to $x$:
\[
\begin{array}{rrrcl}
2x&-3u^2\frac{\del u}{\del x}&+2v\frac{\del v}{\del x} &=& 0\\
2y&-4u\frac{\del u}{\del x}&+12v^3\frac{\del v}{\del x} &=& 0\\
\end{array}
\]
Solving this first equation for $\frac{\del v}{\del x}$ gives 
$$\frac{\del v}{\del x} = \frac{3u^2}{2v}\frac{\del u}{\del x}-\frac{x}{v},$$
and we can substitute this into the second equation to find 
$$\frac{\del u}{\del x}=\frac{6v^2x-y}{9v^2u^2-2u}$$
and we are done. \qed

\end{enumerate}
\end{document}
