\documentclass[letterpaper]{article}
%\documentclass[a5paper]{article}

%% Language and font encodings
\usepackage[english]{babel}
\usepackage[utf8x]{inputenc}
\usepackage[T1]{fontenc}

%% Sets page size and margins
\usepackage[letterpaper,top=1in,bottom=1in,left=1in,right=1in,marginparwidth=1.75cm]{geometry}
%\usepackage[a5paper,top=1cm,bottom=1cm,left=1cm,right=1.5cm,marginparwidth=1.75cm]{geometry}

\input{../tskpreamble}

\pgfplotsset{compat=1.13}

\title{Math 462 - Advanced Linear Algebra \linebreak
	Assignment 2}
\author{Trevor Klar}

\begin{document}

\maketitle

\noindent \textbf{Exercises:}
\begin{enumerate}
\item Let $T: V \to V'$ be a surjective linear transformation of finite-dimensional vector spaces. Show that there exists a subspace $W$ of $V$ such that
$$V = \text{Ker}(T) \oplus W \text{ with } W\cong V'.$$

\begin{proof}
Let $\{v_1, \ldots, v_n\}$ be a basis for $\text{Ker}(T)$. Now extend this basis so that it spans $V$, as follows: $\{v_1, \ldots, v_n, w_1, \ldots, w_k\}$. Now, $\{v_1, \ldots, v_n\} \subset \text{Ker}(T)$, so $T(\{v_1, \ldots, v_n\})=0$. This means that, since $\{v_1, \ldots, v_n, w_1, \ldots, w_k\}$ spans $V$ and $T$ is surjective, then $T(\{v_1, \ldots, v_n, w_1, \ldots, w_k\})=T(\{w_1, \ldots, w_k\})\cup\{0\}$ spans $V'$. Thus, $\{w_1, \ldots, w_k\}$ spans some $W\subset V$ and $T(\{w_1, \ldots, w_k\})\cup\{0\}$ spans $V'$, so $w\cong V'$. 
\end{proof}

\item Let $k$ be a field. Let $\{0\}$ denote the zero vector space over $k$. A sequence of vector spaces of the form 
$$\{0\}\xrightarrow{\alpha_0}V_1\xrightarrow{\alpha_1}V_2\xrightarrow{\alpha_2}\ldots\xrightarrow{\alpha_{n-1}}V_n\xrightarrow{\alpha_n}\{0\}$$
where each $\alpha_i$ is a $k$-linear transformation with im$(a_i)=\ker(a_{i+1})$ is called an \emph{exact sequence}. 

Show that $\sum\limits_{i=0}^n(-1)^i\dim V_i=0$. 

\begin{proof}
\[
\begin{array}{rcl}
\sum\limits_{i=0}^n(-1)^i\dim V_i&=&\sum\limits_{i=0}^n(-1)^i\dim (\text{im}\alpha_i)+\sum\limits_{i=0}^n(-1)^i\dim (\text{ker}\alpha_i) \quad \text{(By Rank-Nullity Thm)}\\ 

&=&\sum\limits_{i=0}^n(-1)^i\dim (\text{ker}\alpha_{i+1})+\sum\limits_{i=0}^n(-1)^i\dim (\text{ker}\alpha_i)\quad \text{(Substitution)}\\ 

&=&\sum\limits_{i=1}^{n+1}(-1)^{i-1}\dim (\text{ker}\alpha_{i})+\sum\limits_{i=0}^n(-1)^i\dim (\text{ker}\alpha_i)\quad \text{(Change of index)}\\ 

&=&(-1)^{n}\dim (\text{ker}\alpha_{n+1}) + \sum\limits_{i=1}^{n}(-1)^{i-1}\dim (\text{ker}\alpha_{i})+ \sum\limits_{i=0}^n(-1)^i\dim (\text{ker}\alpha_i) + \dim (\text{ker}\alpha_{0})\\ 

&=&(-1)^{n}\dim (\text{im}\alpha_{n}) + \sum\limits_{i=1}^{n}(-1)^{i-1}\dim (\text{ker}\alpha_{i})+ \sum\limits_{i=0}^n(-1)^i\dim (\text{ker}\alpha_i) + \dim (\text{ker}\alpha_{0})\\

&=&0 + \left(\sum\limits_{i=1}^{n}(-1)^{i-1}\dim (\text{ker}\alpha_{i})+ \sum\limits_{i=0}^n(-1)^i\dim (\text{ker}\alpha_i)\right) + 0\\

&=&0
\end{array}
\]
\end{proof}

\end{enumerate}
\end{document}