\documentclass[letterpaper]{article}
%\documentclass[a5paper]{article}

%% Language and font encodings
\usepackage[english]{babel}
\usepackage[utf8x]{inputenc}
\usepackage[T1]{fontenc}


%% Sets page size and margins
\usepackage[letterpaper,top=.75in,bottom=1in,left=1in,right=1in,marginparwidth=1.75cm]{geometry}
%\usepackage[a5paper,top=1cm,bottom=1cm,left=1cm,right=1.5cm,marginparwidth=1.75cm]{geometry}

\usepackage{graphicx}
%\graphicspath{../images}	  %%where to look for images

\input{../tskpreamble}

\pgfplotsset{compat=1.13}

%\newcommand{\T}{\mathcal{T}}
%\newcommand{\B}{\mathcal{B}}

%These commands are now in tskpreamble_nothms.tex, but are left as a comment here for reference.
%\newcommand{\arbcup}[1]{\bigcup\limits_{\alpha\in\Gamma}#1_\alpha}
%\newcommand{\arbcap}[1]{\bigcap\limits_{\alpha\in\Gamma}#1_\alpha}
%\newcommand{\arbcoll}[1]{\{#1_\alpha\}_{\alpha\in\Gamma}}
%\newcommand{\arbprod}[1]{\prod\limits_{\alpha\in\Gamma}#1_\alpha}
%\newcommand{\finitecoll}[1]{#1_1, \ldots, #1_n}
%\newcommand{\finitefuncts}[2]{#1(#2_1), \ldots, #1(#2_n)}
%\newcommand{\abs}[1]{\left|#1\right|}
%\newcommand{\norm}[1]{\left|\left|#1\right|\right|}

\title{Math 460 \linebreak
Homework 3}
\author{Trevor Klar}

\begin{document}

\maketitle

\begin{enumerate}
  \item Show that $\langle2-i\rangle$ (that is, the ideal generated by $2 - i$) is maximal in $\Z[i]$ by following these steps:
  	\begin{enumerate}[label=\alph*.]
  	\item Define a map $\phi:\Z\to\Z[i]/\langle2-i\rangle$ by $\phi(n)=n+\langle2-i\rangle$. Show $\phi$ is a ring homomorphism.
  	\begin{proof}\mbox{}
  		\begin{itemize}
  		\item Since $\phi(1)=1+\langle2-i\rangle$, then $\phi$ maps unity to unity.
  		\item Let $a, b \in \Z$. Then
  		$$\phi(a+b)=(a+b)+\langle2-i\rangle=\big(a+\langle2-i\rangle\big)+\big(b+\langle2-i\rangle\big)=\phi(a)+\phi(b).$$
  		\item Let $a, b \in \Z$. Then
  		$$\phi(ab)=(ab)+\langle2-i\rangle=\big(a+\langle2-i\rangle\big)\big(b+\langle2-i\rangle\big)=\phi(a)\phi(b).$$
  		\end{itemize}
  		Thus $\phi$ is a ring homomorphism.
  	\end{proof}

  	\item Now show $\phi$ is onto.
  	\begin{proof}
  		Let $(a+bi)+\langle2-i\rangle\in \Z[i]/\langle2-i\rangle$ be given. Choose $n=a+2b$. This means that
  		$$\phi(n)=\phi(a+2b)=(a+2b)+\langle2-i\rangle=(a+bi)+\langle2-i\rangle.$$
  		To see that this last equality holds, observe that
  		$$(a+2b)-(a+bi)=2b-bi=b(2-i)\in\langle2-i\rangle.$$
  		Therefore we can produce an integer which $\phi$ maps to any element of $\Z[i]/\langle2-i\rangle$, so $\phi$ is onto.
  	\end{proof}

  	\item Show $\ker\phi=5\Z$.
  	\begin{proof} \textbf{($\ker\phi\supseteq5\Z$)}
  %	We will show both directions at once.
  	Observe that $2+\langle2-i\rangle=i+\langle2-i\rangle$. Then for all $5n\in5\Z$, %and $k\in\ker\phi$,
  	\[\begin{array}{rcl}
  	\phi(5n)&=&5n+\langle2-i\rangle\\
  	&=&(2^2+1)n+\langle2-i\rangle\\
  	&=&(i^2+1)n+\langle2-i\rangle\\
  	&=&\langle2-i\rangle\\
  %	&=&\phi(k).
  	\end{array}\]
  	Thus, $5\Z\subseteq\ker\phi$.
  	\end{proof}
  	\begin{proof}\textbf{($\ker\phi\subseteq5\Z$)} Let $k\in\ker\phi$ be given. Then $k\in\langle2-i\rangle$, so there exists $a,b\in\Z$ such that
  	$$k=(a+bi)(2-i)=(2a+b)+(-a+2b)i,$$
  	which implies that $a=2b$, and $k=2a+b$. Thus
  	\[\begin{array}{rcl}
  	k&=&2a+b\\
  	&=&2(2b)+b\\
  	&=&5b.\\
  	\end{array}\]
  	Therefore, for all $k\in\ker\phi$, we can find $b\in\Z$ such that $k=5b$, so $\ker\phi\subseteq5\Z$.
  	\end{proof}

  	\item Now, use the FHT. \\
  	Therefore, since $\phi:\Z\to\Z[i]/\langle2-i\rangle$ is onto and $\ker\phi=5\Z$, then
  	$$\Z/5\Z=\Z_5\cong\Z[i]/\langle2-i\rangle$$
  	by the FHT. Since $\Z_5$ is a field, then so is $\Z[i]/\langle2-i\rangle$, which means that $\langle2-i\rangle$ is a maximal ideal in $\Z[i]$. \qed
  	\end{enumerate}

  \item Show that $\langle3-i\rangle$ (that is, the ideal generated by $3 - i$) is not prime in $\Z[i]$ by following these steps:
	\begin{enumerate}[label=\alph*.]
  	\item Define $\phi:\Z\to\Z[i]/\langle3-i\rangle$ by $\phi(n)=n+\langle3-i\rangle$. Show $\phi$ is an onto ring homomorphism.
  	\begin{proof}\mbox{}
    	\begin{itemize}
    		\item Since $\phi(1)=1+\langle3-i\rangle$, then $\phi$ maps unity to unity.
    		\item Let $a, b \in \Z$. Then
    		$$\phi(a+b)=(a+b)+\langle3-i\rangle=\big(a+\langle3-i\rangle\big)+\big(b+\langle3-i\rangle\big)=\phi(a)+\phi(b).$$
    		\item Let $a, b \in \Z$. Then
    		$$\phi(ab)=(ab)+\langle3-i\rangle=\big(a+\langle3-i\rangle\big)\big(b+\langle3-i\rangle\big)=\phi(a)\phi(b).$$
    		\item Let $(a+bi)+\langle3-i\rangle\in\Z[i]/\langle3-i\rangle$ be given. Choose $n=a+3b$. Then since $$(a+3b)-(a+bi)=b(3-i)\in\langle3-i\rangle,$$ then $$\phi(n)=(a+3b)+\langle3-i\rangle=(a+bi)+\langle3-i\rangle.$$
    	\end{itemize}
    	Therefore, $\phi$ is an onto homomorphism.
  	\end{proof}
    \item Show $\ker\phi=10\Z$.
    \begin{proof}\textbf{($\ker\phi\supseteq10\Z$)} 
    	Let $10n\in10\Z$ be given. Observe that $3+\langle3-i\rangle=i+\langle3-i\rangle$. Then 
    	\[\begin{array}{rcl}
    	\phi(10n)&=&10n+\langle3-i\rangle\\
    	&=&(3^2+1)n+\langle3-i\rangle\\
    	&=&(i^2+1)n+\langle3-i\rangle\\
    	&=&\langle3-i\rangle\\
    	\end{array}\]
			Thus $10\Z\subseteq\ker\phi$.
    \end{proof}
    \begin{proof}\textbf{($\ker\phi\subseteq10\Z$)} 
    	Let $k\in\ker\phi$ be given. Then $k\in\langle3-i\rangle$, which means that there exists $a,b\in\Z$ such that 
    	$$k=(a+bi)(3-i)=(3a+b)+(3b-a)i,$$
    	which means that $a=3b$ and $k=3a+b$. Thus
    	\[\begin{array}{rcl}
   		k&=&3a+b\\
   		&=&3(3b)+b\\
   		&=&10b\\
    	\end{array}\]
			Therefore, $\ker\phi\subseteq10\Z$. 
    \end{proof}
  	\item By FHT, $$\Z/10\Z=\Z_{10}\cong\Z[i]/\langle3-i\rangle,$$ so $\langle3-i\rangle$ is not prime.
  	\begin{proof}
  		If $\langle3-i\rangle$ were prime, then $\Z[i]/\langle3-i\rangle$ would be an integral domain. However, $\Z_{10}$ has zero divisors ($2\times5=0$), so neither ring is an integral domain, so $\langle3-i\rangle$ is not prime.
  	\end{proof}
  \end{enumerate}
	\pagebreak  
  \item Define $N:\Z[\sqrt{6}]\to\Z$ by $N\big(a+b\sqrt{6}\big) = a^2-6b^2.$
  \begin{enumerate}[label=\alph*.]
  	\item Show that $N$ is multiplicative, i.e. $N(xy)=N(x)N(y)$ for all $x,y\in\Z[\sqrt{6}].$
  	\begin{proof}
  		Let $x,y\in\Z[\sqrt{6}]$ be given. Then we can write $x=a+b\sqrt{6}$ and $y=c+d\sqrt{6}$. Then 
  		\[\begin{array}{rcl}
  			N(xy)&=&N\big((a+b\sqrt{6})(c+d\sqrt{6})\big)\\
  			&=&N\big((ac+6bd)+(ad+bc)\sqrt{6}\big)\\
  			&=&a^2c^2+12abcd+36b^2d^2 - 6a^2d^2-12abcd-6b^2c^2\\
  			&=&a^2c^2-6a^2d^2-6b^2c^2+36b^2d^2\\
  			&=&(a^2-6b^2)(c^2-6d^2)\\
  			&=&N(a+b\sqrt{6})N(c+d\sqrt{6})\\
  			&=&N(x)N(y)
  		\end{array}\]
  		and we are done.
  	\end{proof}
  	\item Use $N$ to explain why the only invertible elements in $\Z[\sqrt{6}]$ have $N$ of 1.
  	\begin{proof}\textbf{($\implies$)}
  		Let $x\in\Z[\sqrt{6}]$ be invertible. Then there exists $y\in\Z[\sqrt{6}]$ such that $xy=1$. Taking $N$ of both sides, we find that
  		$$N(x)N(y)=N(xy)=N(1)=1.$$
  		Since $N(x),N(y)\in\Z$, then $N(x)=N(y)=\pm1$. This means that if $x=a+b\sqrt{6}$, then 
  		$$a^2-6b^2=\pm1.$$
  		This second-order Diophantine equation has no solutions for the negative case, but infinitely many for the positive, i.e. $N(1)=N(-1)=N(5+2\sqrt6)=N(5-2\sqrt6)=1$. Thus, any invertible element $x\in\Z[\sqrt{6}]$ is such that $N(x)=1$. 
  	\end{proof}
  	\begin{proof}\textbf{($\impliedby$)}
  		Let $x\in\Z[\sqrt{6}]$ with $N(x)=1$. Then if we write $x=(a+b\sqrt6)$, choose $y=(a-b\sqrt6)$. Then 
  		$$xy=(a+b\sqrt6)(a-b\sqrt6)=a^2-6b^2=N(x)=1,$$
  		so $xy=1$ and $x$ is invertible. 
  	\end{proof}
  	\item Show that $\sqrt6$ is not an irreducible element in $\Z[\sqrt6]$ by writing it as a product of two non-invertible elements in $\Z[\sqrt6]$. 
  	\begin{proof}
  		Since $N(\sqrt{6})=-6$, we have that $\sqrt6$ is nonzero and not a unit. However, 
  		$$(2+\sqrt6)(3-\sqrt6)=\sqrt6,$$ so $\sqrt6$ is reducible. To confirm this, we check that $(2+\sqrt6)$ and $(3-\sqrt6)$ are non-units. $N(2+\sqrt6)=-2$ and $N(3-\sqrt6)=3$, and we know that $N(x)=1$ for all $x\in U\big(\Z[\sqrt{6}]\big)$, so we are done. 
  	\end{proof}
  	\item Prove that $(1+\sqrt6)$ is irreducible in $\Z[\sqrt6]$. 
  	\begin{proof}
  		Suppose $x, y\in \Z[\sqrt6]$ such that $xy=(1+\sqrt6)$. Then 
  		$$N(x)N(y)=N(1+\sqrt6)=-5.$$
  		Since $N(x),N(y)\in\Z$, Then $N(x),N(y)$ are 1,-5 or -1,5. We know already that there are no elements of $\Z[\sqrt6]$ with $N$ of -1, so that means that either $N(x)=1$ or $N(y)=1$, and thus one of them is a unit. 
  	\end{proof}
  	\item Prove that $(1+\sqrt6)$ is prime in $\Z[\sqrt6]$. 
  	\begin{proof}
	  	Suppose $(1+\sqrt6)=ab$ for some $a,b\in\Z[\sqrt6]$. Since $(1+\sqrt6)$ is irreducible, then either $a$ or $b$ is a unit. If $a$ is invertible, then $a^{-1}(1+\sqrt6)=a^{-1}ab=b$, so $(1+\sqrt6)|b$. Otherwise if $b$ is invertible, then $(1+\sqrt6)b^{-1}=abb^{-1}=a$, so $(1+\sqrt6)|a$.
  	\end{proof}
  \end{enumerate}
	\pagebreak  
  \item Show that the domains $\Z[\sqrt{-6}]$ and $\Z[\sqrt{-7}]$ are not UFDs. Just look at how we did $\Z[\sqrt{-3}]$ in class.
  \textbf{Lemma} The only units of $\Z[\sqrt{-n}]$ where $1<n\in\Z$ are $\pm1$. 
  \begin{proof}
  	Consider $\eta:\Z[\sqrt{-n}]\to\N$ defined by $\eta(a+b\sqrt{-n})=a^2+nb^2$. $\eta$ is multiplicative for the same reasons as in (3a), so for any units $x,y$ we have that $\eta(x)\eta(y)=\eta(1)=1$. If we write $x=(a+b\sqrt{-n})$, then 
  	$$\eta(x)=a^2+nb^2=1,$$
  	which can only hold for $b=0$, $a=\pm1$ (since $a,b\in\Z$). 
  \end{proof}
 	Now we prove that $\Z[\sqrt{-6}]$ and $\Z[\sqrt{-7}]$ are not UFDs. 
 	\begin{enumerate}[label=\alph*.]
 		\item \textbf{Claim.} $\Z[\sqrt{-6}]$ is not a UFD, because 
 		$(2+\sqrt{-6})(2-\sqrt{-6})=10=(5)(2)$
 		and all of $2, 5, (2\pm\sqrt{-6})$ are irreducible. 
 		\begin{proof}
 			To see that $(2+\sqrt{-6})$ is irreducible, observe that $(2+\sqrt{-6})\neq\pm1$ and thus is not a unit and nonzero. Suppose $xy=(2+\sqrt{-6})$ where $x,y\in\Z[\sqrt{-6}]$ are not units. Then $\eta(x)\eta(y)=\eta(2+\sqrt{-6})=10$, so 
 			$$\eta(x)=(a^2+6b^2)=5,2.$$
 			This has no solutions, since $(a^2+6b^2)>5$ for $b\neq0$ and $5,2$ are not square numbers. By the same argument, $(2-\sqrt{-6})$ is irreducible as well. \\
 			A similar argument shows that $5$ is irreducible. Observe that $5\neq\pm1$ and thus is not a unit and nonzero. Suppose $xy=$ where $x,y\in\Z[\sqrt{-6}]$ are not units. Since $\eta(5)=\eta(5+6\sqrt{-6})=25$, then 
 			$$\eta(x)=(a^2+6b^2)=5, $$
 			and we have already seen that this has no solutions. The same argument shows that $2$ is also irreducible.
 		\end{proof}
 		\item \textbf{Claim.} $\Z[\sqrt{-7}]$ is not a UFD, because $(1+\sqrt{-7})(1-\sqrt{-7})=8=2^3$ and all of $2, (1\pm\sqrt{-7})$ are irreducible. 
		\begin{proof}
	 		We use a similar proof as in (4a), and omit some notation. To see that $(1+\sqrt{-7})$ is irreducible, observe that $(1+\sqrt{-7})\neq\pm1$ and $\eta(x)\eta(y)=8$, so 
 			$$\eta(x)=(a^2+7b^2)=2,4. $$
 			Though $(2+0\sqrt{-7})$ is a solution to $\eta(x)=4$, there are no solutions to $\eta(x)=2$, so there is no such $x\in\Z[\sqrt{-7}]$ such that $2x=(1+\sqrt{-7})$. Thus we conclude that $(1+\sqrt{-7})$ is irreducible, and so is $(1-\sqrt{-7})$, since it has the same $\eta$. Also $2$ is irreducible by the same reasoning as in the previous problem. 
 		\end{proof}		 			
 	\end{enumerate}
\end{enumerate}
\end{document}
